IMP-/IMP_Minus_Nat_Bijection.thy
@@ -13,11 +13,11 @@ lemma xxx: "x \<noteq> y \<Longrightarrow> (s (x := aval a s)) y = s y"
   by (auto simp add: Assign eval_nat_numeral)
 *)
 
-unbundle IMP_Minus_Minus_Com.no_com_syntax
+(*unbundle IMP_Minus_Minus_Com.no_com_syntax
 
-unbundle Com.no_com_syntax
+unbundle Com.no_com_syntax*)
 
-record triangle_state = triangle_mul_state::mul_state triangle_a::nat triangle_triangle::nat
+record triangle_state = triangle_a::nat triangle_triangle::nat
 
 term Nat_Bijection.triangle
 
@@ -36,11 +36,10 @@ definition "triangle_state_upd (s::triangle_state) \<equiv>
         mul_a' = triangle_a s;
         mul_b' = (triangle_a s) + 1;
         mul_c' = 0;
-        mul_d' = 0;
-        (triangle_mul_state::mul_state) = \<lparr>mul_a = mul_a', mul_b = mul_b', mul_c = mul_c', mul_d = mul_d'\<rparr>;
+        (triangle_mul_state::mul_state) = \<lparr>mul_a = mul_a', mul_b = mul_b', mul_c = mul_c'\<rparr>;
         mul_ret = (mul_imp triangle_mul_state);
         triangle_triangle = (mul_c mul_ret) div 2;
-        ret = \<lparr>triangle_mul_state = mul_ret, triangle_a = triangle_a s,triangle_triangle = triangle_triangle\<rparr>
+        ret = \<lparr>triangle_a = triangle_a s,triangle_triangle = triangle_triangle\<rparr>
       in
         ret
 "
@@ -71,9 +70,7 @@ fun triangle_imp_time:: "nat \<Rightarrow> triangle_state \<Rightarrow> nat" whe
      t = t + 2;
      mul_c' = 0;
      t = t + 2;
-     mul_d' = 0;
-     t = t + 2;
-     (triangle_mul_state::mul_state) = \<lparr>mul_a = mul_a', mul_b = mul_b', mul_c = mul_c', mul_d = mul_d'\<rparr>;
+     (triangle_mul_state::mul_state) = \<lparr>mul_a = mul_a', mul_b = mul_b', mul_c = mul_c'\<rparr>;
      mul_ret = (mul_imp triangle_mul_state);
      t = t + mul_imp_time 0 triangle_mul_state;
      triangle_triangle = mul_c mul_ret div 2;
@@ -91,22 +88,20 @@ lemma triangle_imp_time_acc: "(triangle_imp_time (Suc t) s) = Suc (triangle_imp_
   by (induction t s rule: triangle_imp_time.induct)
      (auto simp add: triangle_imp_time.simps mul_state_upd_def Let_def eval_nat_numeral split: if_splits)
 
-definition triangle_IMP_minus where
-"triangle_IMP_minus \<equiv>
+definition triangle_IMP_Minus where
+"triangle_IMP_Minus \<equiv>
   (
    \<comment> \<open>mul_a' = triangle_a s;\<close>
-   [''mul''] ''a'' ::= (A (V ''a'')) ;;
+   (''mul'' @ ''a'') ::= (A (V ''a'')) ;;
    \<comment> \<open>mul_b' = (triangle_a s) + 1;\<close>
-   [''mul''] ''b'' ::= ((V ''a'') \<oplus> (N 1));;
+   (''mul'' @ ''b'') ::= ((V ''a'') \<oplus> (N 1));;
    \<comment> \<open>mul_c' = 0;\<close>
-   [''mul''] ''c'' ::= (A (N 0)) ;;
-   \<comment> \<open>mul_d' = 0;\<close>
-   [''mul''] ''d'' ::= (A (N 0));;
-   \<comment> \<open>(mul_state::mul_state) = \<lparr>mul_a = mul_a, mul_b = mul_b, mul_c = 0, mul_d = 0\<rparr>;\<close>
+   (''mul'' @  ''c'') ::= (A (N 0)) ;;
+   \<comment> \<open>(mul_state::mul_state) = \<lparr>mul_a = mul_a, mul_b = mul_b, mul_c = 0\<rparr>;\<close>
    \<comment> \<open>mul_ret = (mul_imp mul_state);\<close>
    invoke_subprogram ''mul'' mul_IMP_minus;;
    \<comment> \<open>triangle_triangle = mul_c mul_ret div 2;\<close>
-  ''triangle'' ::= [''mul''] ((V ''c'') \<then>);;
+  ''triangle'' ::= (V (''mul'' @ ''c'') \<then>);;
   ''a'' ::= A (V ''a'')
   )"
 
@@ -116,8 +111,7 @@ definition triangle_IMP_minus where
  (mul_IMP_Minus_state_transformer (''mul'' @ p) (triangle_mul_state s))"*)
 
 definition "triangle_imp_to_HOL_state p s =
-              \<lparr>triangle_mul_state = mul_imp_to_HOL_state (p @ ''mul'') s, 
-               triangle_a = s (add_prefix p ''a''), triangle_triangle = (s (add_prefix p ''triangle''))\<rparr>"
+              \<lparr>triangle_a = s (add_prefix p ''a''), triangle_triangle = (s (add_prefix p ''triangle''))\<rparr>"
 
 lemma triangle_imp_to_HOL_state_add_prefix: 
   "triangle_imp_to_HOL_state (add_prefix p1 p2) s = triangle_imp_to_HOL_state p2 (s o (add_prefix p1))"
@@ -141,14 +135,14 @@ lemma cons_append: "xs \<noteq> [] \<Longrightarrow> x # xs = [x] @ xs"
   by simp
 
 lemma triangle_IMP_Minus_correct_function: 
-  "(triangle_IMP_minus p, s) 
+  "(invoke_subprogram p triangle_IMP_Minus, s) 
       \<Rightarrow>\<^bsup>t \<^esup> s'
     \<Longrightarrow> s' (add_prefix p ''triangle'') = triangle_triangle (triangle_imp (triangle_imp_to_HOL_state p s))"
-  apply(simp only: triangle_IMP_minus_def triangle_imp.simps)
+  apply(simp only: triangle_IMP_Minus_def triangle_imp.simps com_add_prefix.simps invoke_subprogram_append)
   apply(erule Seq_tE)+
   \<comment> \<open>Variables that we want to preserve: variables of this program minus the variables of the
      program we call. If automation fails, this should be manually chosen variables.\<close>
-  apply(simp only: comp_def, erule mul_IMP_minus_correct'[where vars = "{''traingle''}"])
+  apply(erule mul_IMP_minus_correct[where vars = "{''traingle''}"])
   apply(drule AssignD)+
   apply(elim conjE impE)
   apply(auto simp: triangle_state_upd_def Let_def triangle_imp_to_HOL_state_def)[1]
@@ -156,15 +150,15 @@ lemma triangle_IMP_Minus_correct_function:
   done
 
 lemma triangle_IMP_Minus_correct_time: 
-  "(triangle_IMP_minus p, s) 
+  "(invoke_subprogram p triangle_IMP_Minus, s) 
       \<Rightarrow>\<^bsup>t\<^esup> s'
     \<Longrightarrow> t = triangle_imp_time 0 (triangle_imp_to_HOL_state p s)"
-  apply(simp only: triangle_IMP_minus_def)
+  apply(simp only: triangle_IMP_Minus_def com_add_prefix.simps invoke_subprogram_append)
   apply(erule Seq_tE)+
    apply(drule AssignD)+
    apply(elim conjE)
    apply(subst triangle_imp_time.simps)
-  apply(subst (asm) comp_def, erule mul_IMP_minus_correct'[where vars = "(set (all_variables (triangle_IMP_minus p))) - (set (all_variables (mul_IMP_minus p)))"])
+  apply(erule mul_IMP_minus_correct[where vars = "{''triangle''}"])
   \<comment> \<open>Warning: in the following, I am unfolding mul_imp_to_HOL_state_def. With more experiments, it
       should become clear if this will cascade down multiple layers\<close>
   apply(simp add: triangle_imp_time_acc triangle_imp_to_HOL_state_def triangle_state_upd_def)[1]
@@ -172,17 +166,145 @@ lemma triangle_IMP_Minus_correct_time:
   done
 
 lemma triangle_IMP_Minus_correct_effects:
-  "(triangle_IMP_minus p, s) \<Rightarrow>\<^bsup>t\<^esup> s' \<Longrightarrow> (vars \<inter> set (all_variables (triangle_IMP_minus p)) = {} \<longrightarrow> (\<forall>v\<in>vars. s v = s' v))"
-  by (auto intro: com_only_vars)
+  "(invoke_subprogram (p @ triangle_pref) triangle_IMP_Minus, s) \<Rightarrow>\<^bsup>t\<^esup> s' \<Longrightarrow> p @ v \<in> vars \<Longrightarrow> \<not> (set triangle_pref \<subseteq> set v) \<Longrightarrow> s (add_prefix p v) = s' (add_prefix p v)"
+  using com_add_prefix_valid_subset com_only_vars
+  by blast
 
-lemma triangle_IMP_minus_correct':
-  "\<lbrakk>(triangle_IMP_minus p, s) \<Rightarrow>\<^bsup>t\<^esup> s';
-     \<lbrakk>t = (triangle_imp_time 0 (triangle_imp_to_HOL_state p s));
-      s' (add_prefix p ''triangle'') = triangle_triangle (triangle_imp (triangle_imp_to_HOL_state p s));
-      (vars \<inter> set (all_variables (triangle_IMP_minus p)) = {} \<Longrightarrow> (\<forall>v\<in>vars. s v = s' v))\<rbrakk>
+lemma triangle_IMP_Minus_correct:
+  "\<lbrakk>(invoke_subprogram (p1 @ p2) triangle_IMP_Minus, s) \<Rightarrow>\<^bsup>t\<^esup> s';
+     \<lbrakk>t = (triangle_imp_time 0 (triangle_imp_to_HOL_state (p1 @ p2) s));
+      s' (add_prefix (p1 @ p2) ''triangle'') = triangle_triangle (triangle_imp (triangle_imp_to_HOL_state (p1 @ p2) s));
+      \<And>v. p1 @ v \<in> vars \<Longrightarrow> \<not> (set p2 \<subseteq> set v) \<Longrightarrow> s (add_prefix p1 v) = s' (add_prefix p1 v)\<rbrakk>
      \<Longrightarrow> P\<rbrakk> \<Longrightarrow> P"
   using triangle_IMP_Minus_correct_time triangle_IMP_Minus_correct_function
-        triangle_IMP_Minus_correct_effects
+        triangle_IMP_Minus_correct_effects 
+  by auto
+
+record prod_encode_state = prod_encode_a::nat prod_encode_b::nat prod_encode_ret::nat
+
+(*  [''a''] ''a'' ::= ((V ''a'') \<oplus> (V ''b'')) ;;
+  invoke_subprogram ''a'' triangle_IMP_Minus ;;
+  ''prod_encode'' ::= [''a''] (A (V ''triangle'')) ;;
+  [''a''] ''triangle'' ::= (A (N 0)) ;;
+  ''prod_encode'' ::= ((V ''a'') \<oplus> (V ''prod_encode''))"*)
+
+definition "prod_encode_state_upd (s::prod_encode_state) \<equiv>
+      let
+        triangle_a = prod_encode_a s + prod_encode_b s;
+        triangle_triangle' = 0;
+        (triangle_state::triangle_state) = \<lparr>triangle_a = triangle_a, triangle_triangle = triangle_triangle'\<rparr>;
+        triangle_ret = (triangle_imp triangle_state);
+        prod_encode_ret = triangle_triangle triangle_ret;
+        prod_encode_ret = prod_encode_ret + prod_encode_a s;
+        ret = \<lparr>prod_encode_a = prod_encode_a s,prod_encode_b = prod_encode_b s, prod_encode_ret = prod_encode_ret\<rparr>
+      in
+        ret
+"
+
+fun prod_encode_imp:: "prod_encode_state \<Rightarrow> prod_encode_state" where
+"prod_encode_imp s = 
+  (let
+     ret = prod_encode_state_upd s
+   in
+     ret
+  )"
+
+lemmas [simp del] = prod_encode_imp.simps
+
+lemma prod_encode_imp_correct: "prod_encode_ret (prod_encode_imp s) = prod_encode (prod_encode_a s, prod_encode_b s)"
+proof (induction s rule: prod_encode_imp.induct)
+  case (1 s)
+  then show ?case
+    by (auto simp: prod_encode_imp.simps prod_encode_def prod_encode_state_upd_def Let_def triangle_imp_correct split: if_splits)
+qed 
+
+fun prod_encode_imp_time:: "nat \<Rightarrow> prod_encode_state \<Rightarrow> nat" where
+"prod_encode_imp_time t s = 
+  (let
+     triangle_a = prod_encode_a s + prod_encode_b s;
+     t = t + 2;
+     triangle_triangle' = 0;
+     t = t + 2;
+     (triangle_state::triangle_state) = \<lparr>triangle_a = triangle_a, triangle_triangle = triangle_triangle'\<rparr>;
+     triangle_ret = (triangle_imp triangle_state);
+     t = t + triangle_imp_time 0 triangle_state;
+     prod_encode_ret = triangle_triangle triangle_ret;
+     t = t + 2;
+     prod_encode_ret = prod_encode_ret + prod_encode_a s;
+     t = t + 2;
+     ret = t
+   in
+     ret
+  )"
+
+lemmas [simp del] = prod_encode_imp_time.simps
+
+lemma prod_encode_imp_time_acc: "(prod_encode_imp_time (Suc t) s) = Suc (prod_encode_imp_time t s)"
+  by (induction t s rule: prod_encode_imp_time.induct)
+     (auto simp add: prod_encode_imp_time.simps Let_def eval_nat_numeral split: if_splits)
+
+(*        triangle_a = prod_encode_a s + prod_encode_b s;
+        (triangle_state::triangle_state) = \<lparr>triangle_a = triangle_a, triangle_triangle = 0\<rparr>;
+        triangle_ret = (triangle_imp triangle_state);
+        prod_encode_ret = triangle_triangle triangle_ret + prod_encode_a s;
+*)
+
+definition prod_encode_IMP_Minus where "prod_encode_IMP_Minus \<equiv>
+  (''triangle.'' @ ''a'') ::= ((V ''a'') \<oplus> (V ''b'')) ;;
+  (''triangle.'' @ ''triangle'') ::= (A (N 0)) ;;
+  invoke_subprogram ''triangle.'' triangle_IMP_Minus ;;
+  ''prod_encode'' ::= (A (V (''triangle.'' @ ''triangle''))) ;;
+  ''prod_encode'' ::= ((V ''a'') \<oplus> (V ''prod_encode''))"
+
+definition "prod_encode_imp_to_HOL_state p s =
+  \<lparr>prod_encode_a = s (add_prefix p ''a''), prod_encode_b = s (add_prefix p ''b''), prod_encode_ret = (s (add_prefix p ''prod_encode''))\<rparr>"
+
+lemma notD: "x \<notin> s \<Longrightarrow> (x \<in> s \<Longrightarrow> False)"
+  by auto
+
+lemma prod_encode_IMP_Minus_correct_function: 
+  "(invoke_subprogram p prod_encode_IMP_Minus, s) 
+      \<Rightarrow>\<^bsup>t \<^esup> s'
+    \<Longrightarrow> s' (add_prefix p ''prod_encode'') = prod_encode_ret (prod_encode_imp (prod_encode_imp_to_HOL_state p s))"
+  apply(simp only: prod_encode_IMP_Minus_def prod_encode_imp.simps com_add_prefix.simps invoke_subprogram_append)
+  apply(erule Seq_tE)+
+  \<comment> \<open>Variables that we want to preserve: variables of this program minus the variables of the
+     program we call. If automation fails, this should be manually chosen variables.\<close>
+  apply(erule triangle_IMP_Minus_correct[where vars = "{p @ ''a''}"])
+  apply(drule AssignD)+
+  apply(elim conjE impE)
+  apply(auto simp: prod_encode_state_upd_def Let_def prod_encode_imp_to_HOL_state_def)[1]
+  apply(auto simp: triangle_imp_to_HOL_state_def)[1]
+  done
+
+lemma prod_encode_IMP_Minus_correct_time: 
+  "(invoke_subprogram p prod_encode_IMP_Minus, s) 
+      \<Rightarrow>\<^bsup>t\<^esup> s'
+    \<Longrightarrow> t = prod_encode_imp_time 0 (prod_encode_imp_to_HOL_state p s)"
+  apply(simp only: prod_encode_IMP_Minus_def prod_encode_imp_time.simps com_add_prefix.simps invoke_subprogram_append)
+  apply(erule Seq_tE)+
+  \<comment> \<open>Variables that we want to preserve: variables of this program minus the variables of the
+     program we call. If automation fails, this should be manually chosen variables.\<close>
+  apply(erule triangle_IMP_Minus_correct[where vars = "{p @ ''a''}"])
+  apply(drule AssignD)+
+  apply(elim conjE impE)
+  apply(auto simp: prod_encode_state_upd_def Let_def prod_encode_imp_to_HOL_state_def)[1]
+  apply(auto simp: triangle_imp_to_HOL_state_def)[1]
+  done
+
+lemma prod_encode_IMP_Minus_correct_effects:
+  "(invoke_subprogram (p @ prod_encode_pref) prod_encode_IMP_Minus, s) \<Rightarrow>\<^bsup>t\<^esup> s' \<Longrightarrow> p @ v \<in> vars \<Longrightarrow> \<not> (set prod_encode_pref \<subseteq> set v) \<Longrightarrow> s (add_prefix p v) = s' (add_prefix p v)"
+  using com_add_prefix_valid_subset com_only_vars
+  by blast
+
+lemma prod_encode_IMP_Minus_correct:
+  "\<lbrakk>(invoke_subprogram (p1 @ p2) prod_encode_IMP_Minus, s) \<Rightarrow>\<^bsup>t\<^esup> s';
+     \<lbrakk>t = (prod_encode_imp_time 0 (prod_encode_imp_to_HOL_state (p1 @ p2) s));
+      s' (add_prefix (p1 @ p2) ''prod_encode'') = prod_encode_ret (prod_encode_imp (prod_encode_imp_to_HOL_state (p1 @ p2) s));
+      \<And>v. p1 @ v \<in> vars \<Longrightarrow> \<not> (set p2 \<subseteq> set v) \<Longrightarrow> s (add_prefix p1 v) = s' (add_prefix p1 v)\<rbrakk>
+     \<Longrightarrow> P\<rbrakk> \<Longrightarrow> P"
+  using prod_encode_IMP_Minus_correct_time prod_encode_IMP_Minus_correct_function
+        prod_encode_IMP_Minus_correct_effects 
   by auto
 
 end
